# Negatives

$$sin(-\theta) = -sin \theta$$
$$cos(- \theta) = -cos \theta$$
$$tan(- \theta) = - tan \theta$$
$$cosec(- \theta) = - cosec \theta$$
$$sec(- \theta) = - sec \theta$$
$$cot(- \theta) = - cot \theta$$
# Product to Sum
$$sinx \cdot siny = \frac{1}{2}[cos(x-y) - cos(x+y)]$$
$$cosx \cdot cosy = \frac{1}{2}[cos(x-y) + cos(x+y)$$
$$sinx \cdot cosy = \frac{1}{2}[sin(x+y) + sin(x-y)]$$
$$cosx \cdot siny = \frac{1}{2}[sin(x+y) - sin(x - y)]$$
# Sum to Product
$$sinx + siny = 2sin\frac{(x+y)}{2}  \cdot cos\frac{(x-y)}{2}$$
$$sin x - sin y = 2 cos \frac{(x+y)}{2}\cdot sin\frac{(x-y)}{2}$$
$$cos x + cos y = 2cos \frac{(x + y)}{2}\cdot cos\frac{(x-y)}{2}$$
$$cos x - cos y = -2 sin\frac{(x + y)}{2} \cdot sin\frac{(x-y)}{2}$$
# Identities
$$sin^2A + cos^2A = 1$$
$$1 + tan^2A = sec^2A$$
$$1 + cot^2A = cosec^2 A$$
# Addition
$$cos( A + B) = cosA\cdot cosB - sinA\cdot sinB$$
$$cos(A - B) = cosA\cdot cosB + sinA\cdot sinB$$
$$sin(A + B) = sinA\cdot cosB + cosA\cdot sinB$$
$$sin(A - B) = sinA\cdot cosB - cosA\cdot sinB$$
$$tan(A + B) = \frac{tanA + tanB}{1 - tanA\cdot tanB}$$
$$tan(A - B) = \frac{tan A - tanB}{1 + tanA\cdot tanB}$$
$$cot(A + B) = \frac{cotA\cdot cotB - 1}{cotB + cotA}$$
$$cot(A - B) = \frac{cotA\cdot cotB + 1}{cotB - cotA}$$
# Sum formulas
$$cos(A + B)\cdot cos(A - B) = cos^2A - sin^2B = cos^2B - sin^2A$$
$$sin(A + B)\cdot sin(A - B) = sin^2A - sin^2B = cos^2B - cos^2A$$
$$
$$
# Twice
$$sin2A = 2sinA\cdot cosA = \frac{2tanA}{1 + tan^2A}$$
$$cos2A = cos^2A - sin^2A = 1-2sin^2A = 2cos^2A - 1 = \frac{1-tan^2A}{1 + tan^2A}$$
$$tan2A = \frac{2tanA}{1-tan^2A}$$
# Triple
$$sin3A = 3sinA - 4sin^3A$$
$$cos3A = 4cos^3A - 3cosA$$
$$tan3A = \frac{3tanA - tan^3A}{1-3tan^2A}$$

# Compound
$$sin(A + B) + sin(A - B) = 2sinA\cdot cosB$$
$$sin(A + B) - sin(A - B) = 2cosA\cdot sinB$$
$$cos(A + B) + cos(A - B) = 2cosA\cdot cosB$$
$$cos(A + B) - cos(A - B) = -2sinA\cdot sinB$$

$$sinC + sinD = 2sin \frac{C + D}{2}\cdot cos\frac{C-D}{2}$$
$$sinC - sin D = 2cos \frac{C+D}{2}\cdot sin\frac{C-D}{2}$$
$$cos C + cos D = 2cos\frac{C + D}{2}\cdot cos\frac{C-D}{2}$$
$$cos C - cos D = 2sin \frac{C+D}{2}\cdot sin\frac{C-D}{2}$$
# Derivative
$$\frac{d}{dx}(\sin x) = \cos x$$
$$\frac{d}{dx}(\cos x) = - \sin x$$
$$\frac{d}{dx}(\tan x) = \sec^2 x$$
$$\frac{d}{dx}(\cot x) = - \csc ^2 x$$
$$\frac{d}{dx}(\csc) = - \csc \cdot \cot x$$
$$\frac{d}{dx}(\sec x) = \sec x \cdot \tan x$$

# Derivative Inverse
$$\frac{d}{dx}(\sin^{-1}x) = \frac{1}{\sqrt{1 - x^2}}$$
$$\frac{d}{dx}(\cos ^{-1} x) = \frac{-1}{\sqrt{1-x^2}}$$
$$\frac{d}{dx}(\tan ^{-1} x) = \frac{1}{\sqrt{1+x^2}}$$
$$\frac{d}{dx}(\cot ^{-1} x) = \frac{-1}{\sqrt{1+x^2}}$$
$$\frac{d}{dx}(\sec^{-1}x)=\frac{1}{x\sqrt{x^2-1}}$$
$$\frac{d}{dx}(\csc^{-1}x)=\frac{1}{x\sqrt{x^2 - 1}}$$